@prefix : <http://www.gsi.upm.es/ontologies/sebb/ns#> .
@prefix amor: <http://www.gsi.upm.es/ontologies/amor/ns#> .
@prefix concept: <http://sw.opencyc.org/concept/> .
@prefix dc: <http://purl.org/dc/terms/> .
@prefix mls: <http://www.w3.org/ns/mls#> .
@prefix oro: <http://kb.openrobots.org#> .
@prefix owl: <http://www.w3.org/2002/07/owl#> .
@prefix prov: <http://www.w3.org/ns/prov#> .
@prefix rdfs: <http://www.w3.org/2000/01/rdf-schema#> .
@prefix vann: <http://purl.org/vocab/vann/> .
@prefix xsd: <http://www.w3.org/2001/XMLSchema#> .

<http://www.gsi.upm.es/ontologies/sebb/ns>
  a owl:Ontology ;
  rdfs:label "Semantic Ethical Black Box (SEBB) Ontology"@en ;
  owl:versionInfo "1.0.0"^^xsd:string ;
  owl:versionIRI <http://www.gsi.upm.es/ontologies/sebb/ns/1.0.0> ;
  dc:title "Semantic Ethical Black Box (SEBB) Ontology"@en ;
  dc:creator "√Ålvaro Carrera Barroso"@en ;
  dc:publisher <http://www.gsi.upm.es> ;
  rdfs:comment "SEBB is an ontology designed for representing logging information generated by different sources in a common Semantic Ethical Black Box."@en ;
  dc:description "SEBB is an ontology designed for representing logging information generated by different sources in a common Semantic Ethical Black Box."@en ;
  vann:preferredNamespacePrefix "sebb" ;
  vann:preferredNamespaceUri "http://www.gsi.upm.es/ontologies/sebb/ns#" .

:LoggedActivity
    a owl:Class ;
    rdfs:subClassOf prov:Activity ;
    owl:unionOf (
        concept:Action 
        oro:RobotResponses 
        oro:Intent 
        mls:Run
    ) ;
    rdfs:label "Logged Activity"@en ;
    rdfs:comment "Represents an activity that is recorded/logged in the SEBB."@en .

:Trigger
    a owl:Class ;
    owl:unionOf (
        prov:Entity 
        prov:Activity
    ) ;
    rdfs:label "Trigger"@en ;
    rdfs:comment "Represents an event that caused/triggered an activity."@en .

:Result
    a owl:Class ;
    rdfs:subClassOf prov:Activity ;
    owl:unionOf (
        prov:Entity 
        prov:Activity
    ) ;
    rdfs:label "Result"@en ;
    rdfs:comment "Represents the result of an activity."@en .

:triggeredBy
    a owl:ObjectProperty ;
    rdfs:subPropertyOf prov:wasInfluencedBy ;
    rdfs:domain :LoggedActivity ;
    rdfs:range :Trigger ;
    rdfs:label "triggered by"@en ;
    rdfs:comment "Represents the relation between an activity and the event which triggered it."@en .

:triggeredByActivity
    a owl:ObjectProperty ;
    rdfs:subPropertyOf :triggeredBy ;
    rdfs:domain :LoggedActivity ;
    rdfs:range [
        a owl:Class ;
        owl:intersectionOf (
            prov:Activity
            :Trigger
        )
    ] ;
    rdfs:label "triggered by activity"@en ;
    rdfs:comment "Represents the relation between an activity and the event which triggered it, where the event is an activity."@en .

:triggeredByEntity
    a owl:ObjectProperty ;
    rdfs:subPropertyOf :triggeredBy ;
    rdfs:domain :LoggedActivity ;
    rdfs:range [
        a owl:Class ;
        owl:intersectionOf (
            prov:Entity
            :Trigger
        )
    ] ;
    rdfs:label "triggered by entity"@en ;
    rdfs:comment "Represents the relation between an activity and the event which triggered it, where the event is an entity."@en .

:intermediateActivity
    a owl:ObjectProperty ;
    prov:subPropertyOf prov:wasInfluencedBy ;
    rdfs:domain :LoggedActivity ;
    rdfs:range :LoggedActivity ;
    rdfs:label "intermediate activity"@en ;
    rdfs:comment "Represents the relation between a logged activity and another activity that is an intermediate step towards the final result."@en .
:producedResult
    a owl:ObjectProperty ;
    rdfs:subPropertyOf prov:wasInfluencedBy ;
    rdfs:domain :LoggedActivity ;
    rdfs:range :Result ;
    rdfs:label "produced result"@en ;
    rdfs:comment "Represents the relation between a result and an activity which produced it."@en .

:producedActivityResult
    a owl:ObjectProperty ;
    rdfs:subPropertyOf :producedResult ;
    rdfs:domain :LoggedActivity ;
    rdfs:range [
        a owl:Class ;
        owl:intersectionOf (
            prov:Activity
            :Result
        )
    ] ;
    rdfs:label "produced activity result"@en ;
    rdfs:comment "Represents the relation between a result and an activity which produced it, where the result is an activity."@en .

:producedActivityEntity
    a owl:ObjectProperty ;
    rdfs:subPropertyOf :producedResult ;
    rdfs:domain :LoggedActivity ;
    rdfs:range [
        a owl:Class ;
        owl:intersectionOf (
            prov:Entity
            :Result
        )
    ] ;
    rdfs:label "produced activity entity"@en ;
    rdfs:comment "Represents the relation between a result and an activity which produced it, where the result is an entity."@en .

:usedMLModel
    a owl:ObjectProperty ;
    rdfs:subPropertyOf prov:used ;
    owl:equivalentProperty amor:usedMLModel ;
    rdfs:domain prov:Activity ;
    rdfs:range mls:Model ;
    rdfs:label "used machine learning model"@en ;
    rdfs:comment "Represents the fact that an activity has used a Machine Learning Model to produce the result."@en .
